04-14-2021.v
@@ -1,0 +1,116 @@
+Module Note.
+
+  (* Syntax: *)
+
+  Inductive Exp : Type :=
+  | T
+  | F
+  | And (b1 : Exp) (b2 : Exp)       
+  | If  (b : Exp)  (b1 : Exp) (b2 : Exp).
+
+  Notation "b1 /*\ b2" := (And b1 b2) (at level 50, left associativity).
+
+  Definition exp1 : Exp := T.
+  Definition exp2 : Exp := T /*\ F.
+  Definition exp3 : Exp := If exp2 (T /*\ T) F.  
+
+  (* An indexed data type (b is the index): 
+      isVal T 
+      isVal F
+  *)
+  Inductive isVal : Exp -> Prop :=
+  | valT : isVal T
+  | valF : isVal F.
+
+  (* Parameterized Data Type (b is the parameter): *)
+  Inductive isVal' (b : Exp) : Prop :=
+  | valT' : b = T -> isVal' b
+  | valF' : b = F -> isVal' b.
+
+  (* Evaluation: Single and Multi *)
+
+  Fixpoint eval (b : Exp) : Exp :=
+    match b with
+    | T => T
+    | F => F
+    | T /*\ T => T (* AndT  *)
+    | F /*\ T => F (* AndF1 *)
+    | T /*\ F => F (* AndF2 *)
+    | F /*\ F => F (* AndF  *)
+    | b1 /*\ b2 =>
+      match (eval b1) with
+      | T => eval b2
+      | F => F
+      | _ => b1 /*\ b2
+      end
+    | If b b1 b2 =>
+      match eval b with
+      | T => eval b1
+      | F => eval b2
+      | _ => If b b1 b2
+      end       
+    end.
+
+  Lemma isval_to_val : forall (b : Exp),
+      isVal b -> b = T \/ b = F.
+  Proof.
+    intros.
+    destruct H.
+    left.
+    trivial.
+    right.
+    trivial.
+  Qed. 
+
+  Lemma eval_T : forall (b : Exp),
+   eval b = T ->
+     (b = T)
+  \/ (exists (b1 b2 : Exp), b = b1 /*\ b2)
+  \/ (exists (b1 b2 b3 : Exp), b = If b1 b2 b3).
+  Proof.
+    intros.
+    destruct b.  
+    - left. trivial.
+    - left. trivial.
+    - right. left. exists b1. exists b2. trivial.
+    - right. right. exists b1. exists b2. exists b3. trivial.
+  Qed.
+  
+  Lemma eval_and : forall (b1 b2 : Exp),
+        (eval b1 = T \/ eval b1 = F) ->
+        (eval b2 = T \/ eval b1 = F) ->
+        (eval (b1 /*\ b2) = T \/ eval (b1 /*\ b2) = F).
+  Proof.
+    intros.
+    destruct H.
+    - destruct H0.
+      left.
+      simpl.
+      rewrite H.
+      rewrite H0.
+      destruct (eval_T b1).
+      * apply H.
+      * rewrite H1. destruct (eval_T b2).
+      + apply H0.
+      + rewrite H2. trivial.
+      +  destruct H2.
+         { destruct H2. destruct H2. rewrite H2. trivial. }
+         { destruct H2. destruct H2. destruct H2. rewrite H2. trivial. }
+      *  
+           
+  Lemma eval_to_val : forall (b : Exp), isVal (eval b).
+  Proof. 
+    intro b.
+    induction b.
+    apply valT.
+    apply valF.
+    
+    (* isVal (eval b1) -> eval b1 = T \/ eval b1 = F
+    * isVal (eval b2) -> eval b2 = T \/ eval b1 = F 
+    * ---------------------------------------------
+    * eval (b1 /*\ b2) = T \/ eval (b1 /*\ b2) = F  *)
+    
+
+  Compute (eval (If (T /*\ T) (F /*\ T) T)).
+
+End Note.
